lib/Lib.Buffer.fsti
@@ -821,6 +821,19 @@ val fill:
       modifies1 o h h' /\
       as_seq h' o == Seq.createi #a (v clen) (spec h0))
 
+inline_for_extraction noextract
+let eq_or_disjoint
+    (#t1:buftype)
+    (#t2:buftype)
+    (#a1:Type)
+    (#a2:Type)
+    (#clen1:size_t)
+    (#clen2:size_t)
+    (b1:lbuffer_t t1 a1 clen1)
+    (b2:lbuffer_t t2 a2 clen2) =
+    disjoint b1 b2 \/
+    (t1 == t2 /\ a1 == a2 /\ clen1 == clen2 /\ b1 == b2)
+
 (** Map a total function onto a buffer *)
 inline_for_extraction
 val mapT:
@@ -836,6 +849,24 @@ val mapT:
     (ensures  fun h0 _ h1 ->
       modifies1 o h0 h1 /\
       as_seq h1 o == Seq.map f (as_seq h0 i))
+
+inline_for_extraction
+val map2T:
+    #t:buftype
+  -> #a1:Type
+  -> #a2:Type
+  -> #b:Type
+  -> clen:size_t
+  -> o:lbuffer b clen
+  -> f:(a1 -> a2 -> Tot b)
+  -> i1:lbuffer_t t a1 clen
+  -> i2:lbuffer_t t a2 clen ->
+  Stack unit
+    (requires fun h0 -> live h0 o /\ live h0 i1 /\ live h0 i2 /\
+                     eq_or_disjoint o i1 /\ eq_or_disjoint o i2)
+    (ensures  fun h0 _ h1 ->
+      modifies1 o h0 h1 /\
+      as_seq h1 o == Seq.map2 f (as_seq h0 i1) (as_seq h0 i2))
 
 (** Map a total function (depending on the index) onto a buffer *)
 inline_for_extraction
@@ -871,3 +902,39 @@ val mapi:
     (ensures  fun h _ h1 ->
       modifies1 o h h1 /\
       as_seq h1 o == Seq.mapi (spec_f h0) (as_seq h i))
+
+
+inline_for_extraction noextract
+val map_blocks:
+    #t:buftype
+  -> #a:Type0
+  -> h0: mem
+  -> len:size_t
+  -> blocksize:size_t{v blocksize > 0}
+  -> inp:lbuffer_t t a len
+  -> output:lbuffer a len
+  -> spec_f:(mem -> GTot (i:nat{i < v len / v blocksize} -> Seq.lseq a (v blocksize) -> Seq.lseq a (v blocksize)))
+  -> spec_l:(mem -> GTot (i:nat{i == v len / v blocksize} -> llen:size_nat{llen < v blocksize} -> Seq.lseq a llen -> Seq.lseq a llen))
+  -> impl_f:(i:size_t{v i < v len / v blocksize} -> Stack unit
+      (requires fun h1 ->
+        (v i + 1) * v blocksize <= max_size_t /\
+        modifies (loc (gsub output 0ul (i *! blocksize))) h0 h1)
+      (ensures  fun h1 _ h2 ->
+        let iblock = gsub inp (i *! blocksize) blocksize in
+        let oblock = gsub output (i *! blocksize) blocksize in
+        let ob = spec_f h0 (v i) (as_seq h1 iblock) in
+        B.modifies (loc oblock) h1 h2 /\
+        as_seq h2 oblock == ob))
+  -> impl_l:(i:size_t{v i == v len / v blocksize} -> Stack unit
+      (requires fun h1 ->
+        modifies (loc (gsub output 0ul (i *! blocksize))) h0 h1)
+      (ensures  fun h1 _ h2 ->
+        let iblock = gsub inp (i *! blocksize) (len %. blocksize)  in
+        let oblock = gsub output (i *! blocksize) (len %. blocksize) in
+        let ob = spec_l h0 (v i) (v len % v blocksize) (as_seq h1 iblock) in
+        B.modifies (loc oblock) h1 h2 /\
+        as_seq h2 oblock == ob))
+  -> Stack unit
+    (requires fun h -> h0 == h /\ live h output /\ live h inp /\ eq_or_disjoint inp output)
+    (ensures  fun _ _ h1 -> modifies1 output h0 h1 /\
+        (admit (); as_seq h1 output == Seq.map_blocks (v blocksize) (as_seq h0 inp) (spec_f h0) (spec_l h0)))
