lib/Lib.LoopCombinators.fst
@@ -44,6 +44,14 @@ let unfold_repeati #a n f acc0 i =
 let repeat #a n f acc0 =
   repeati n (fun i -> f) acc0
 
+let eq_repeat0 #a f acc0 = ()
+
+let fixed_i f (i:nat) = f
+
+let unfold_repeat #a n f acc0 i =
+  admit ();
+  unfold_repeati #a n (fixed_i f) acc0 i
+
 let repeat_range #a min max f x =
   repeat_left min max (fun _ -> a) f x
 
